src/M/PlutusTx.lean
@@ -1,0 +1,9 @@
+
+
+import M.PlutusTx.AssocMap
+
+
+namespace PlutusTx
+
+
+end PlutusTx
