src/M/PlutusTx/AssocMap.lean
@@ -1,0 +1,45 @@
+
+
+namespace PlutusTx.AssocMap
+
+
+structure Map (k v) where
+  toList : List (k × v)
+deriving Inhabited, Repr
+
+
+private def insertPair [BEq k] : List (k × v) → (k × v) → List (k × v)
+  | []                       , entry        => [entry]
+  | (key', value') :: entries, (key, value) => if key == key'
+                                                 then (key , value ) :: entries
+                                                 else (key', value') :: insertPair entries (key, value)
+
+
+namespace Map
+
+  def empty : Map k v :=
+    mk []
+
+  def fromList [BEq k] : List (k × v) → Map k v :=
+    mk ∘ List.foldl insertPair default
+
+  def insert [BEq k] : k → v → Map k v → Map k v 
+    | key, value, mk entries => mk $ insertPair entries (key, value)
+
+
+  def lookup [BEq k] [Inhabited v] : k → Map k v → v
+    | _  , mk []                          => default
+    | key, mk ((key', value') :: entries) => if key == key'
+                                               then value'
+                                               else lookup key $ mk entries
+
+  def member [BEq k]: k → Map k v → Bool
+    | _  , mk []                     => false
+    | key, mk ((key', _) :: entries) => if key == key'
+                                          then true
+                                          else member key $ mk entries
+
+end Map
+
+
+end PlutusTx.AssocMap
